theories/SpecNotations.v
@@ -2,9 +2,9 @@ Require Import Blech.Spec.
 
 Infix "*" := t_prod.
 
-Notation "Γ ⊢ E 'in' t" := (JE Γ E t) (at level 90).
-Notation "⊢ v 'in' t" := (Jv v t) (at level 90).
+Notation "Γ ⊢ E ? t" := (JE Γ E t) (at level 90).
+Notation "Γ ⊢ v 'in' t" := (Jv Γ v t) (at level 90).
 
-Notation "v0 ⇓ v1" := (big v0 v1) (at level 90).
+Notation "v ⇓ N" := (big v N) (at level 90).
 
 Infix "|-" := P_with (at level 30).
